{
  "@context": {
    "schema": "http://schema.org/",
    "rdf": "http://www.w3.org/1999/02/22-rdf-syntax-ns#",
    "rdfs": "http://www.w3.org/2000/01/rdf-schema#",
    "bioschema": "http://discovery.biothings.io/view/bioschema/"
  },
  "@graph": [
    {
      "@id": "bioschema:Taxon",
      "@type": "rdfs:Class",
      "rdfs:comment": "A set of organisms asserted to represent a natural cohesive biological unit.",
      "rdfs:label": "Taxon",
      "rdfs:subClassOf": {
        "@id": "schema:Thing"
      },
      "$validation": {
        "$schema": "http://json-schema.org/draft-07/schema#",
        "type": "object",
        "properties": {
          "childTaxon": {
            "description": "Closest child taxa of the taxon in question. Inverse property: parentTaxon",
            "oneOf": [
              {
                "type": "string"
              },
              {
                "type": "string",
                "format": "uri"
              },
              {
                "@type": "bioschema:Taxon",
                "type": "object",
                "properties": {},
                "required": []
              }
            ]
          },
          "hasDefinedTerm": {
            "description": " \tA Defined Term contained in this term set.",
            "@type": "DefinedTerm",
            "type": "object",
            "properties": {},
            "required": []
          },
          "parentTaxon": {
            "description": "Closest parent taxon of the taxon in question. Inverse property: childTaxon",
            "oneOf": [
              {
                "type": "string"
              },
              {
                "type": "string",
                "format": "uri"
              },
              {
                "@type": "bioschema:Taxon",
                "type": "object",
                "properties": {},
                "required": []
              }
            ]
          },
          "taxonRank": {
            "description": "The taxonomic rank of this taxon given preferably as a URI from a controlled vocabulary \u2013 (typically the ranks from TDWG TaxonRank ontology or equivalent Wikidata URIs). ",
            "oneOf": [
              {
                "type": "string"
              },
              {
                "type": "string",
                "format": "uri"
              },
              {
                "@type": "PropertyValue",
                "type": "object",
                "properties": {},
                "required": []
              }
            ]
          }
        },
        "required": []
      }
    },
    {
      "@id": "bioschema:childTaxon",
      "@type": "rdf:Property",
      "rdfs:comment": "Closest child taxa of the taxon in question. Inverse property: parentTaxon",
      "rdfs:label": "childTaxon",
      "schema:domainIncludes": {
        "@id": "bioschema:Taxon"
      },
      "schema:rangeIncludes": [
        {
          "@id": "bioschema:Taxon"
        },
        {
          "@id": "schema:Text"
        },
        {
          "@id": "schema:URL"
        }
      ]
    },
    {
      "@id": "bioschema:hasDefinedTerm",
      "@type": "rdf:Property",
      "rdfs:comment": " \tA Defined Term contained in this term set.",
      "rdfs:label": "hasDefinedTerm",
      "schema:domainIncludes": {
        "@id": "bioschema:Taxon"
      },
      "schema:rangeIncludes": [
        {
          "@id": "schema:DefinedTerm"
        }
      ]
    },
    {
      "@id": "bioschema:parentTaxon",
      "@type": "rdf:Property",
      "rdfs:comment": "Closest parent taxon of the taxon in question. Inverse property: childTaxon",
      "rdfs:label": "parentTaxon",
      "schema:domainIncludes": {
        "@id": "bioschema:Taxon"
      },
      "schema:rangeIncludes": [
        {
          "@id": "bioschema:Taxon"
        },
        {
          "@id": "schema:Text"
        },
        {
          "@id": "schema:URL"
        }
      ]
    },
    {
      "@id": "bioschema:taxonRank",
      "@type": "rdf:Property",
      "rdfs:comment": "The taxonomic rank of this taxon given preferably as a URI from a controlled vocabulary \u2013 (typically the ranks from TDWG TaxonRank ontology or equivalent Wikidata URIs). ",
      "rdfs:label": "taxonRank",
      "schema:domainIncludes": {
        "@id": "bioschema:Taxon"
      },
      "schema:rangeIncludes": [
        {
          "@id": "schema:PropertyValue"
        },
        {
          "@id": "schema:Text"
        },
        {
          "@id": "schema:URL"
        }
      ]
    }
  ]
}